src/Tom_proof.thy
@@ -35,17 +35,67 @@ apply(thin_tac "ni = _")
 apply(simp add: wellformed_ts_def)
 apply(simp add: dest_ts_def)
 apply(elim conjE)
+apply(case_tac n)
+apply(rename_tac ks rs)
+apply(simp)
 apply(intro conjI)
  (* wf_focus *)
  apply(simp add: wellformed_focus_def )
- apply()
+ apply(case_tac f)
+  (* inserting_one *)
+  apply(rename_tac t)
+  apply(simp)
+  apply(simp add: update_focus_at_position_def)
+  apply(subgoal_tac "wellformed_subtree (Node (ks,rs))")
+   apply(force intro:FIXME)
+  apply(simp add: wellformed_subtree_def)
+  apply(intro conjI)
+   apply(simp add: wf_size_def)
+   apply(force intro:FIXME)
+   
+   apply(force intro:FIXME)
+
+   apply(force intro:FIXME)
+
+   (* keys_consistent; but tihs follows from wf_ts *)
+   apply(force intro:FIXME)
+
+   apply(force intro:FIXME)
+
+  (* inserting_two *)
+  apply(simp)
+  apply(case_tac x2)
+  apply(rename_tac tleft k0 tr)
+  apply(simp add: update_focus_at_position_def)
+  apply(elim conjE)
+  apply(thin_tac "x2 = _")
+  apply(subgoal_tac "? ks2.  list_insert_at_n (n |> fst) i [k0] = ks2") prefer 2 apply(force)
+  apply(subgoal_tac "? rs2. list_replace_at_n (n |> snd) i [tleft, tr] |> dest_Some = rs2") prefer 2 apply(force)
+  apply(elim exE)
+  apply(simp add: Let_def)
+  apply(case_tac "length ks2 \<le> max_node_keys")
+   apply(simp)
+   apply(force intro: FIXME)
+
+   apply(simp)
+   apply(simp add: split_node_def)
+   apply(force intro: FIXME)
+  
 
  (* wf_context *)
-
+ apply(force intro: FIXME)
 
   (* wf_ts_1 *)
+  apply(simp add: update_focus_at_position_def)
+  apply(case_tac f)
+   (* i1 *)
+   apply(simp)
+   apply(force intro: FIXME)
 
-end
+   (* i2 FIXME may be worth combining with other i2 cases? *)
+   apply(simp)
+   apply(force intro: FIXME)
+done
 
 
 end
